trying to define MachineWidth_XLEN in terms of coqutil.Word

src/MachineWidth_XLEN.v
@@ -1,66 +1,96 @@
 Require Import Coq.ZArith.ZArith.
 Require Import Coq.micromega.Lia.
-Require Import riscv.util.Word.
+Require Import coqutil.Word.Interface.
+Require Import coqutil.Word.Properties.
+Require coqutil.Word.Naive.
+Require Import coqutil.Word.LittleEndian.
+Require Import coqutil.Datatypes.HList.
 Require Import riscv.Utility.
 Local Open Scope Z_scope.
 
-Instance MachineWidth_XLEN(sz: Z)(bound: 8 <= sz): MachineWidth (word sz) := {|
-  add := @wadd sz;
-  sub := @wsub sz;
-  mul := @wmul sz;
-  div := @wsquot sz;
-  rem := @wsrem sz;
-  negate := @wopp sz;
-  signed_less_than := @wsltb sz;
-  reg_eqb := @weqb sz;
-  xor := @wxor sz;
-  or := @wor sz;
-  and := @wand sz;
-  XLEN := sz;
-  regToInt8  := wscast 8;
-  regToInt16 := wscast 16;
-  regToInt32 := wscast 32;
-  regToInt64 := wscast 64;
-  uInt8ToReg  := wucast sz;
-  uInt16ToReg := wucast sz;
-  uInt32ToReg := wucast sz;
-  uInt64ToReg := wucast sz;
-  int8ToReg  := wscast sz;
-  int16ToReg := wscast sz;
-  int32ToReg := wscast sz;
-  int64ToReg := wscast sz;
-  s32(x: word sz) := wscast sz (wscast 32 x);
-  u32(x: word sz) := wucast sz (wucast 32 x);
-  regToZ_signed := @swordToZ sz;
-  regToZ_unsigned := @uwordToZ sz;
-  sll w n := ZToWord sz (Z.shiftl (uwordToZ w) n);
-  srl w n := ZToWord sz (Z.shiftr (uwordToZ w) n);
-  sra w n := ZToWord sz (Z.shiftr (swordToZ w) n);
-  ltu := @wultb sz;
-  divu := @wuquot sz;
-  remu := @wurem sz;
-  maxSigned := ZToWord sz (2 ^ (sz - 1) - 1);
-  maxUnsigned := ZToWord sz (2 ^ sz - 1);
-  minSigned := ZToWord sz (- 2 ^ (sz - 1));
-  regToShamt5 x := (uwordToZ x) mod 2 ^ 5;
-  regToShamt  x := (uwordToZ x) mod 2 ^ (Z.log2 sz);
-  highBits x := ZToWord sz (bitSlice x sz (2 * sz));
-  ZToReg := ZToWord sz;
-  regRing := @word_ring sz;
-  ZToReg_morphism := @word_ring_morph_Z sz;
-  reg_eqb_spec := @weqb_spec sz;
-  regToZ_signed_bounds   _ := @swordToZ_bound sz _ ltac:(lia);
-  regToZ_unsigned_bounds _ := @uwordToZ_bound sz _ ltac:(lia);
-  add_def_signed := @wadd_wsadd sz;
-  sub_def_signed := @wsub_wssub sz;
-  mul_def_signed := @wmul_wsmul sz;
-  regToZ_ZToReg_signed := @swordToZ_ZToWord sz;
-  regToZ_ZToReg_unsigned_mod := @uwordToZ_ZToWord sz;
-  ZToReg_regToZ_unsigned := @ZToWord_uwordToZ sz;
-  ZToReg_regToZ_signed := @ZToWord_swordToZ sz;
-  XLEN_lbound := bound;
-  div_def  _ _ := eq_refl;
-  rem_def  _ _ := eq_refl;
-  divu_def _ _ := eq_refl;
-  remu_def _ _ := eq_refl;  
-|}.
+Section M.
+  Variable sz: Z.
+  Hypothesis bound: 8 <= sz.
+  Lemma bound_8 : 0 < 8.  omega. Qed.
+  Lemma bound_sz: 0 < sz. omega. Qed.
+  Lemma bound_sz_le: 0 <= sz. omega. Qed.
+
+  Instance byte: Interface.word 8 := Naive.word 8 bound_8.
+  Instance byte_ok: word.ok byte := Naive.ok _ _.
+  Instance word_sz: Interface.word sz := Naive.word sz bound_sz.
+  Instance word_ok: word.ok word_sz := Naive.ok _ _.
+
+  Set Refine Instance Mode.
+
+  Definition TODO{T: Type}: T. Admitted.
+
+  Instance MachineWidth_XLEN: MachineWidth word_sz := {|
+    w8  := tuple byte 1;
+    w16 := tuple byte 2;
+    w32 := tuple byte 4;
+    w64 := tuple byte 8;
+    add := word.add;
+    sub := word.sub;
+    mul := word.mul;
+    div := word.divs;
+    rem := word.mods;
+    negate := word.opp;
+    signed_less_than := word.lts;
+    reg_eqb := word.eqb;
+    xor := word.xor;
+    or := word.or;
+    and := word.and;
+    XLEN := sz;
+    regToInt8 := split 1;
+    regToInt16 := split 2;
+    regToInt32 := split 4;
+    regToInt64 := split 8;
+    uInt8ToReg  := combine 1;
+    uInt16ToReg := combine 2;
+    uInt32ToReg := combine 4;
+    uInt64ToReg := combine 8;
+    int8ToReg  a := word.sextend  8 (combine 1 a);
+    int16ToReg a := word.sextend 16 (combine 2 a);
+    int32ToReg a := word.sextend 32 (combine 4 a);
+    int64ToReg a := word.sextend 64 (combine 8 a);
+    s32 := word.sextend 32;
+    u32(x: word_sz) := word.of_Z ((word.unsigned x) mod 2 ^ 32);
+    regToZ_signed := word.signed;
+    regToZ_unsigned := word.unsigned;
+    sll w n := word.of_Z (Z.shiftl (word.unsigned w) n);
+    srl w n := word.of_Z (Z.shiftr (word.unsigned w) n);
+    sra w n := word.of_Z (Z.shiftr (word.signed   w) n);
+    ltu := word.ltu;
+    divu := word.divu;
+    remu := word.modu;
+    maxSigned := word.of_Z (2 ^ (sz - 1) - 1);
+    maxUnsigned := word.of_Z (2 ^ sz - 1);
+    minSigned := word.of_Z (- 2 ^ (sz - 1));
+    regToShamt5 x := (word.unsigned x) mod 2 ^ 5;
+    regToShamt  x := (word.unsigned x) mod 2 ^ (Z.log2 sz);
+    highBits x := word.of_Z (bitSlice x sz (2 * sz));
+    ZToReg := word.of_Z;
+    regRing := word.ring_theory bound_sz_le;
+    ZToReg_morphism := word.ring_morph bound_sz_le;
+  |}.
+  all: intros.
+  - apply TODO.
+  - apply word.signed_range. omega.
+  - apply word.unsigned_range. omega.
+  - apply TODO.
+  - apply TODO.
+  - apply TODO.
+  - rewrite word.signed_of_Z. unfold word.swrap. apply TODO.
+  - apply word.unsigned_of_Z.
+  - apply word.of_Z_unsigned.
+  - apply TODO.
+  - assumption.
+  - (* the only lemma which seems reasonable to use here is word.signed_divs,
+       but it doesn't apply *)
+    apply TODO.
+  - apply TODO.
+  - apply TODO.
+  - apply TODO.
+  Defined.
+
+End M.
