src/util/Monads.v
@@ -160,3 +160,19 @@ Module OStateNDOperations.
     forall (o: option (unit * S)), m s o -> exists s', o = Some (tt, s') /\ post s'.
 
 End OStateNDOperations.
+
+Inductive Outcome(A: Type): Type :=
+| Success(a: A)
+| Exception (* recoverable *)
+| HardFailure (* non-recoverable *).
+
+Class ErrorStateMonad(StM: Type -> Type -> Type) := {
+  get{S: Type}: StM S S;
+  put{S: Type}(s: S): StM S unit;
+  throw{S A: Type}: StM S A;
+  failHard{S A: Type}: StM S A;
+  (* not sure if needed here
+  evalState{S A: Type}(m: StM S A): Outcome A;
+  execState{S A: Type}(m: StM S A): Outcome S;
+  *)
+}.
